<?xml version="1.0"?>
<rdf:RDF xmlns="http://www.semanticweb.org/root/ontologies/2018/9/untitled-ontology-7#"
     xml:base="http://www.semanticweb.org/root/ontologies/2018/9/untitled-ontology-7"
     xmlns:rdf="http://www.w3.org/1999/02/22-rdf-syntax-ns#"
     xmlns:owl="http://www.w3.org/2002/07/owl#"
     xmlns:xml="http://www.w3.org/XML/1998/namespace"
     xmlns:xsd="http://www.w3.org/2001/XMLSchema#"
     xmlns:rdfs="http://www.w3.org/2000/01/rdf-schema#">
    <owl:Ontology rdf:about="http://www.semanticweb.org/root/ontologies/2018/9/untitled-ontology-7"/>
    


    <!-- 
    ///////////////////////////////////////////////////////////////////////////////////////
    //
    // Object Properties
    //
    ///////////////////////////////////////////////////////////////////////////////////////
     -->

    


    <!-- http://www.semanticweb.org/root/ontologies/2018/9/untitled-ontology-7#hasMessage -->

    <owl:ObjectProperty rdf:about="http://www.semanticweb.org/root/ontologies/2018/9/untitled-ontology-7#hasMessage">
        <owl:inverseOf rdf:resource="http://www.semanticweb.org/root/ontologies/2018/9/untitled-ontology-7#isFrom"/>
        <rdfs:domain rdf:resource="http://www.semanticweb.org/root/ontologies/2018/9/untitled-ontology-7#Conversation"/>
        <rdfs:range rdf:resource="http://www.semanticweb.org/root/ontologies/2018/9/untitled-ontology-7#Data"/>
    </owl:ObjectProperty>
    


    <!-- http://www.semanticweb.org/root/ontologies/2018/9/untitled-ontology-7#isFrom -->

    <owl:ObjectProperty rdf:about="http://www.semanticweb.org/root/ontologies/2018/9/untitled-ontology-7#isFrom">
        <rdfs:domain rdf:resource="http://www.semanticweb.org/root/ontologies/2018/9/untitled-ontology-7#Data"/>
        <rdfs:range rdf:resource="http://www.semanticweb.org/root/ontologies/2018/9/untitled-ontology-7#Conversation"/>
    </owl:ObjectProperty>
    


    <!-- http://www.semanticweb.org/root/ontologies/2018/9/untitled-ontology-7#participate -->

    <owl:ObjectProperty rdf:about="http://www.semanticweb.org/root/ontologies/2018/9/untitled-ontology-7#participate">
        <rdfs:domain rdf:resource="http://www.semanticweb.org/root/ontologies/2018/9/untitled-ontology-7#ChatBot"/>
        <rdfs:domain rdf:resource="http://www.semanticweb.org/root/ontologies/2018/9/untitled-ontology-7#Person"/>
        <rdfs:range rdf:resource="http://www.semanticweb.org/root/ontologies/2018/9/untitled-ontology-7#Conversation"/>
    </owl:ObjectProperty>
    


    <!-- http://www.semanticweb.org/root/ontologies/2018/9/untitled-ontology-7#sendMessage -->

    <owl:ObjectProperty rdf:about="http://www.semanticweb.org/root/ontologies/2018/9/untitled-ontology-7#sendMessage">
        <owl:equivalentProperty rdf:resource="http://www.semanticweb.org/root/ontologies/2018/9/untitled-ontology-7#store"/>
        <rdfs:domain rdf:resource="http://www.semanticweb.org/root/ontologies/2018/9/untitled-ontology-7#Action"/>
        <rdfs:range rdf:resource="http://www.semanticweb.org/root/ontologies/2018/9/untitled-ontology-7#Data"/>
    </owl:ObjectProperty>
    


    <!-- http://www.semanticweb.org/root/ontologies/2018/9/untitled-ontology-7#store -->

    <owl:ObjectProperty rdf:about="http://www.semanticweb.org/root/ontologies/2018/9/untitled-ontology-7#store">
        <rdfs:domain rdf:resource="http://www.semanticweb.org/root/ontologies/2018/9/untitled-ontology-7#Action"/>
        <rdfs:range rdf:resource="http://www.semanticweb.org/root/ontologies/2018/9/untitled-ontology-7#Data"/>
    </owl:ObjectProperty>
    


    <!-- 
    ///////////////////////////////////////////////////////////////////////////////////////
    //
    // Data properties
    //
    ///////////////////////////////////////////////////////////////////////////////////////
     -->

    


    <!-- http://www.semanticweb.org/root/ontologies/2018/9/untitled-ontology-7#comunicationWay -->

    <owl:DatatypeProperty rdf:about="http://www.semanticweb.org/root/ontologies/2018/9/untitled-ontology-7#comunicationWay">
        <rdfs:domain rdf:resource="http://www.semanticweb.org/root/ontologies/2018/9/untitled-ontology-7#Person"/>
        <rdfs:domain rdf:resource="http://www.semanticweb.org/root/ontologies/2018/9/untitled-ontology-7#SoftwareAplication"/>
        <rdfs:range rdf:resource="http://www.w3.org/2001/XMLSchema#string"/>
        <rdfs:comment xml:lang="en">The comunication way is a &quot;leaf&quot; in my ontology</rdfs:comment>
    </owl:DatatypeProperty>
    


    <!-- http://www.semanticweb.org/root/ontologies/2018/9/untitled-ontology-7#content -->

    <owl:DatatypeProperty rdf:about="http://www.semanticweb.org/root/ontologies/2018/9/untitled-ontology-7#content">
        <rdfs:domain rdf:resource="http://www.semanticweb.org/root/ontologies/2018/9/untitled-ontology-7#Data"/>
        <rdfs:range rdf:resource="http://www.w3.org/2001/XMLSchema#string"/>
    </owl:DatatypeProperty>
    


    <!-- 
    ///////////////////////////////////////////////////////////////////////////////////////
    //
    // Classes
    //
    ///////////////////////////////////////////////////////////////////////////////////////
     -->

    


    <!-- http://www.semanticweb.org/root/ontologies/2018/9/untitled-ontology-7#Action -->

    <owl:Class rdf:about="http://www.semanticweb.org/root/ontologies/2018/9/untitled-ontology-7#Action">
        <rdfs:comment xml:lang="en">&quot;In philosophy, an action is that which is done by an agent. In common speech, the term is often used interchangeably with the term &quot;behaviour&quot;.&quot;</rdfs:comment>
    </owl:Class>
    


    <!-- http://www.semanticweb.org/root/ontologies/2018/9/untitled-ontology-7#Bot -->

    <owl:Class rdf:about="http://www.semanticweb.org/root/ontologies/2018/9/untitled-ontology-7#Bot">
        <rdfs:subClassOf rdf:resource="http://www.semanticweb.org/root/ontologies/2018/9/untitled-ontology-7#SoftwareAplication"/>
        <rdfs:comment xml:lang="pt">&quot;Bot, diminutivo de robot, também conhecido como Internet bot ou web robot, é uma aplicação de software concebido para simular ações humanas repetidas vezes de maneira padrão, da mesma forma como faria um robô.&quot;</rdfs:comment>
    </owl:Class>
    


    <!-- http://www.semanticweb.org/root/ontologies/2018/9/untitled-ontology-7#ChatBot -->

    <owl:Class rdf:about="http://www.semanticweb.org/root/ontologies/2018/9/untitled-ontology-7#ChatBot">
        <rdfs:subClassOf rdf:resource="http://www.semanticweb.org/root/ontologies/2018/9/untitled-ontology-7#Bot"/>
        <owl:disjointWith rdf:resource="http://www.semanticweb.org/root/ontologies/2018/9/untitled-ontology-7#webCrawler"/>
        <rdfs:comment xml:lang="en">&quot;A chatbot (also known as a smartbots, talkbot, chatterbot, Bot, IM bot, interactive agent, Conversational interface or Artificial Conversational Entity) is a computer program or an artificial intelligence which conducts a conversation via auditory or textual methods.&quot;</rdfs:comment>
    </owl:Class>
    


    <!-- http://www.semanticweb.org/root/ontologies/2018/9/untitled-ontology-7#Conversation -->

    <owl:Class rdf:about="http://www.semanticweb.org/root/ontologies/2018/9/untitled-ontology-7#Conversation">
        <rdfs:comment xml:lang="en">&quot;Conversation is interactive communication between two or more people.&quot;</rdfs:comment>
    </owl:Class>
    


    <!-- http://www.semanticweb.org/root/ontologies/2018/9/untitled-ontology-7#Data -->

    <owl:Class rdf:about="http://www.semanticweb.org/root/ontologies/2018/9/untitled-ontology-7#Data">
        <rdfs:comment xml:lang="en">&quot;Data and information are often used interchangeably; however, the extent to which a set of data is informative to someone depends on the extent to which it is unexpected by that person. The amount of information content in a data stream may be characterized by its Shannon entropy.&quot;</rdfs:comment>
    </owl:Class>
    


    <!-- http://www.semanticweb.org/root/ontologies/2018/9/untitled-ontology-7#MessagingAplication -->

    <owl:Class rdf:about="http://www.semanticweb.org/root/ontologies/2018/9/untitled-ontology-7#MessagingAplication">
        <rdfs:subClassOf rdf:resource="http://www.semanticweb.org/root/ontologies/2018/9/untitled-ontology-7#SoftwareAplication"/>
        <rdfs:comment xml:lang="en">&quot;Messaging apps (a.k.a. &quot;Social messaging&quot; or &quot;chat applications&quot;) are apps and platforms that enable messaging, many of which started around social networking platforms,[1] but many of which have now developed into broad platforms enabling status updates, chatbots, payments and conversational commerce (e-commerce via chat).&quot;

I am assuming that chatbots are more than messaging applications because for this ontology, messaging application are just the &quot;way&quot; that the message will pass through.</rdfs:comment>
    </owl:Class>
    


    <!-- http://www.semanticweb.org/root/ontologies/2018/9/untitled-ontology-7#Person -->

    <owl:Class rdf:about="http://www.semanticweb.org/root/ontologies/2018/9/untitled-ontology-7#Person">
        <rdfs:comment xml:lang="en">The objective is to get person from other ontology, like &quot;foaf&quot;.</rdfs:comment>
    </owl:Class>
    


    <!-- http://www.semanticweb.org/root/ontologies/2018/9/untitled-ontology-7#SoftwareAplication -->

    <owl:Class rdf:about="http://www.semanticweb.org/root/ontologies/2018/9/untitled-ontology-7#SoftwareAplication">
        <rdfs:comment xml:lang="en">&quot;An application software (app or application for short) is computer software designed to perform a group of coordinated functions, tasks, or activities for the benefit of the user.&quot;</rdfs:comment>
    </owl:Class>
    


    <!-- http://www.semanticweb.org/root/ontologies/2018/9/untitled-ontology-7#webCrawler -->

    <owl:Class rdf:about="http://www.semanticweb.org/root/ontologies/2018/9/untitled-ontology-7#webCrawler">
        <rdfs:subClassOf rdf:resource="http://www.semanticweb.org/root/ontologies/2018/9/untitled-ontology-7#Bot"/>
        <rdfs:comment xml:lang="en">&quot;A Web crawler, sometimes called a spider or spiderbot and often shortened to crawler, is an Internet bot that systematically browses the World Wide Web, typically for the purpose of Web indexing (web spidering). &quot;</rdfs:comment>
    </owl:Class>
    


    <!-- http://www.semanticweb.org/root/ontologies/2018/9/untitled-ontology-7#webSite -->

    <owl:Class rdf:about="http://www.semanticweb.org/root/ontologies/2018/9/untitled-ontology-7#webSite">
        <rdfs:subClassOf rdf:resource="http://www.semanticweb.org/root/ontologies/2018/9/untitled-ontology-7#SoftwareAplication"/>
        <rdfs:comment xml:lang="en">&quot;A website is a collection of related web pages, including multimedia content, typically identified with a common domain name, and published on at least one web server. Notable examples are wikipedia.org, google.com, and amazon.com. Today roughly 380 new websites are created every minute across the World.&quot;</rdfs:comment>
        <rdfs:comment xml:lang="en">Sarch for webSites ontologies to link here.</rdfs:comment>
    </owl:Class>
    


    <!-- 
    ///////////////////////////////////////////////////////////////////////////////////////
    //
    // Individuals
    //
    ///////////////////////////////////////////////////////////////////////////////////////
     -->

    


    <!-- http://www.semanticweb.org/root/ontologies/2018/9/untitled-ontology-7#Arthur -->

    <owl:NamedIndividual rdf:about="http://www.semanticweb.org/root/ontologies/2018/9/untitled-ontology-7#Arthur">
        <rdf:type rdf:resource="http://www.semanticweb.org/root/ontologies/2018/9/untitled-ontology-7#Person"/>
    </owl:NamedIndividual>
    


    <!-- http://www.semanticweb.org/root/ontologies/2018/9/untitled-ontology-7#Bia -->

    <owl:NamedIndividual rdf:about="http://www.semanticweb.org/root/ontologies/2018/9/untitled-ontology-7#Bia">
        <rdf:type rdf:resource="http://www.semanticweb.org/root/ontologies/2018/9/untitled-ontology-7#ChatBot"/>
    </owl:NamedIndividual>
    


    <!-- http://www.semanticweb.org/root/ontologies/2018/9/untitled-ontology-7#Lino -->

    <owl:NamedIndividual rdf:about="http://www.semanticweb.org/root/ontologies/2018/9/untitled-ontology-7#Lino">
        <rdf:type rdf:resource="http://www.semanticweb.org/root/ontologies/2018/9/untitled-ontology-7#ChatBot"/>
    </owl:NamedIndividual>
    


    <!-- http://www.semanticweb.org/root/ontologies/2018/9/untitled-ontology-7#Taís -->

    <owl:NamedIndividual rdf:about="http://www.semanticweb.org/root/ontologies/2018/9/untitled-ontology-7#Taís">
        <rdf:type rdf:resource="http://www.semanticweb.org/root/ontologies/2018/9/untitled-ontology-7#ChatBot"/>
    </owl:NamedIndividual>
    


    <!-- http://www.semanticweb.org/root/ontologies/2018/9/untitled-ontology-7#facebook -->

    <owl:NamedIndividual rdf:about="http://www.semanticweb.org/root/ontologies/2018/9/untitled-ontology-7#facebook">
        <rdf:type rdf:resource="http://www.semanticweb.org/root/ontologies/2018/9/untitled-ontology-7#MessagingAplication"/>
    </owl:NamedIndividual>
    


    <!-- http://www.semanticweb.org/root/ontologies/2018/9/untitled-ontology-7#rocketchat -->

    <owl:NamedIndividual rdf:about="http://www.semanticweb.org/root/ontologies/2018/9/untitled-ontology-7#rocketchat">
        <rdf:type rdf:resource="http://www.semanticweb.org/root/ontologies/2018/9/untitled-ontology-7#MessagingAplication"/>
    </owl:NamedIndividual>
    


    <!-- http://www.semanticweb.org/root/ontologies/2018/9/untitled-ontology-7#telegram -->

    <owl:NamedIndividual rdf:about="http://www.semanticweb.org/root/ontologies/2018/9/untitled-ontology-7#telegram">
        <rdf:type rdf:resource="http://www.semanticweb.org/root/ontologies/2018/9/untitled-ontology-7#MessagingAplication"/>
    </owl:NamedIndividual>
    


    <!-- http://www.semanticweb.org/root/ontologies/2018/9/untitled-ontology-7#unb -->

    <owl:NamedIndividual rdf:about="http://www.semanticweb.org/root/ontologies/2018/9/untitled-ontology-7#unb">
        <rdf:type rdf:resource="http://www.semanticweb.org/root/ontologies/2018/9/untitled-ontology-7#webSite"/>
    </owl:NamedIndividual>
    


    <!-- http://www.semanticweb.org/root/ontologies/2018/9/untitled-ontology-7#unbRuMenu -->

    <owl:NamedIndividual rdf:about="http://www.semanticweb.org/root/ontologies/2018/9/untitled-ontology-7#unbRuMenu">
        <rdf:type rdf:resource="http://www.semanticweb.org/root/ontologies/2018/9/untitled-ontology-7#webCrawler"/>
    </owl:NamedIndividual>
    


    <!-- http://www.semanticweb.org/root/ontologies/2018/9/untitled-ontology-7#whatsapp -->

    <owl:NamedIndividual rdf:about="http://www.semanticweb.org/root/ontologies/2018/9/untitled-ontology-7#whatsapp">
        <rdf:type rdf:resource="http://www.semanticweb.org/root/ontologies/2018/9/untitled-ontology-7#MessagingAplication"/>
    </owl:NamedIndividual>
    


    <!-- 
    ///////////////////////////////////////////////////////////////////////////////////////
    //
    // General axioms
    //
    ///////////////////////////////////////////////////////////////////////////////////////
     -->

    <rdf:Description>
        <rdf:type rdf:resource="http://www.w3.org/2002/07/owl#AllDisjointClasses"/>
        <owl:members rdf:parseType="Collection">
            <rdf:Description rdf:about="http://www.semanticweb.org/root/ontologies/2018/9/untitled-ontology-7#Action"/>
            <rdf:Description rdf:about="http://www.semanticweb.org/root/ontologies/2018/9/untitled-ontology-7#Conversation"/>
            <rdf:Description rdf:about="http://www.semanticweb.org/root/ontologies/2018/9/untitled-ontology-7#Data"/>
            <rdf:Description rdf:about="http://www.semanticweb.org/root/ontologies/2018/9/untitled-ontology-7#Person"/>
            <rdf:Description rdf:about="http://www.semanticweb.org/root/ontologies/2018/9/untitled-ontology-7#SoftwareAplication"/>
        </owl:members>
    </rdf:Description>
    <rdf:Description>
        <rdf:type rdf:resource="http://www.w3.org/2002/07/owl#AllDisjointClasses"/>
        <owl:members rdf:parseType="Collection">
            <rdf:Description rdf:about="http://www.semanticweb.org/root/ontologies/2018/9/untitled-ontology-7#Bot"/>
            <rdf:Description rdf:about="http://www.semanticweb.org/root/ontologies/2018/9/untitled-ontology-7#MessagingAplication"/>
            <rdf:Description rdf:about="http://www.semanticweb.org/root/ontologies/2018/9/untitled-ontology-7#webSite"/>
        </owl:members>
    </rdf:Description>
</rdf:RDF>



<!-- Generated by the OWL API (version 4.2.8.20170104-2310) https://github.com/owlcs/owlapi -->

